eNFA_Regex_equivalence_other.lean
@@ -75,25 +75,13 @@ noncomputable
 def regex_for_path_from_i_to_j_through_k (A : εNFA α ℕ) (i j k : ℕ) :
     RegularExpression α :=
     if k = 0 then
-        if i = j then
-            let character_set_ii: Finset α := { σ |  i ∈ A.step i (some σ) }
-            let characters_ii := character_set_ii.toList
+        let character_set_ij: Finset α := { σ |  j ∈ A.step i (some σ) }
+        let characters_ij := character_set_ij.toList
 
-            (character_list_to_regex characters_ii).star
-        else if j ∈ A.step i none then
-            let character_set_ij: Finset α := { σ |  j ∈ A.step i (some σ) }
-            let characters_ij := character_set_ij.toList
-            let character_set_jj: Finset α := { σ |  j ∈ A.step j (some σ) }
-            let characters_jj := character_set_jj.toList
-
-            (1 + character_list_to_regex characters_ij) * (character_list_to_regex characters_jj).star
+        if i = j ∨ j ∈ A.step i none then
+            1 + character_list_to_regex characters_ij
         else
-            let character_set_ij: Finset α := { σ |  j ∈ A.step i (some σ) }
-            let characters_ij := character_set_ij.toList
-            let character_set_jj: Finset α := { σ |  j ∈ A.step j (some σ) }
-            let characters_jj := character_set_jj.toList
-
-            character_list_to_regex characters_ij * (character_list_to_regex characters_jj).star
+            character_list_to_regex characters_ij
     else
         let rᵢⱼ := regex_for_path_from_i_to_j_through_k A i j (k-1)
         let rᵢₖ := regex_for_path_from_i_to_j_through_k A i k (k-1)
@@ -217,16 +205,6 @@ lemma path_split_at_state (A : εNFA α ℕ) (qs qf t : ℕ) (x': List (Option �
                         h_t := by simp [h_qs_neq_t, h_supp]
                     }
 
-
-@[simp]
-def εNFA.Path.suppAfterStart
-    {σ : Type*} [DecidableEq σ]
-    {M : εNFA α σ} {s t : σ} {x : List (Option α)} :
-    M.Path s t x → Finset σ
-  | Path.nil _ => ∅
-  | Path.cons _ _ _ _ _ _ p => p.supp
-
-
 structure path_split_full (A : εNFA α ℕ) (i j k : ℕ) (word_ij: List (Option α)) (path_ij: A.Path i j word_ij) where
   word_ik : List (Option α)
   word_kk : List (Option α)
@@ -261,16 +239,10 @@ lemma path_multiple_split_at_state (A : εNFA α ℕ) (i j k : ℕ) (x': List (O
                     path_ik := path_nil
                     path_kk := path_nil
                     path_kj := Path.cons t k j c tail h_step path_tj
-                    h_word_ij := by
-                        simp
-                    h_path_ij := by
-                        cases path_nil
-                        rfl
-                    h_k_notin_ik := by
-                        cases path_nil
-                        simp
-                    h_k_notin_kj := by
-                        simpa [Path.suppAfterStart] using hk_tail
+                    h_word_ij := by simp
+                    h_path_ij := by cases path_nil; rfl
+                    h_k_notin_ik := by cases path_nil; simp
+                    h_k_notin_kj := by simpa [Path.suppAfterStart] using hk_tail
                 }
 
             case pos =>
@@ -328,8 +300,7 @@ lemma path_multiple_split_at_state (A : εNFA α ℕ) (i j k : ℕ) (x': List (O
                     word_kk := [c] ++ word_tk ++ word_kk
                     word_kj := word_kj
                     path_ik := path_ik
-                    path_kk :=
-                        (Path.cons t k k c word_tk h_step path_tk) ++ path_kk
+                    path_kk := (Path.cons t k k c word_tk h_step path_tk) ++ path_kk
                     path_kj := path_kj
                     h_word_ij := by
                         subst tail
@@ -366,811 +337,318 @@ lemma path_multiple_split_at_state (A : εNFA α ℕ) (i j k : ℕ) (x': List (O
                         h_notin_path_kj_tail
                 }
 
-lemma regex_is_path_mp (A : εNFA α ℕ) (i j k : ℕ) (r: RegularExpression α) (hr: r = regex_for_path_from_i_to_j_through_k A i j k)
-    (h_zero_step: ∀ (σ : Option α), A.step 0 σ = ∅) (h_step_zero: ∀ (q : ℕ) (σ : Option α), 0 ∉ A.step q σ):
-    ∀(x : List α), ((x ∈ r.matches') → (∃(x': List ((Option α))), (x'.reduceOption = x) ∧ Nonempty ((to_trim A i j k).Path i j x'))) := by
-    sorry
-    -- intro x h_r_matches_x
-    -- unfold regex_for_path_from_i_to_j_through_k at hr
-    -- split_ifs at hr
-    -- case pos h_k_0 h_ij =>
-    --     subst h_k_0 h_ij
-
-    --     simp [hr, Language.kstar_def] at h_r_matches_x
-    --     cases h_r_matches_x
-    --     case intro L h_L =>
-    --         obtain ⟨ h_x_L, h_L ⟩ := h_L
-
-    --         use [none]
-    --         simp [to_trim]
-    --         split_ifs
-    --         case pos =>
-    --             simp
-
-    --         case neg =>
-    --             simp [h_ij]
-    --             omega
-
-    --     case inr h_x_in_character_list =>
-    --         let character_set: Finset alphabet := { σ |  j ∈ A.step i (some σ) }
-    --         let characters := character_set.toList
-
-    --         obtain ⟨ σ, h_step, h_x_σ ⟩ := (character_list_regex_accepts_characters characters (character_list_to_regex characters) rfl x).mp h_x_in_character_list
-    --         subst characters character_set
-    --         simp at h_step
-
-    --         use [some σ]
-    --         simp [to_trim, h_x_σ]
-    --         split_ifs
-    --         case pos => simp [h_step]
-    --         case neg => simp [h_step] ; omega
-
-    -- case neg h_k_0 =>
-    --     simp [hr] at h_r_matches_x
-    --     let character_set: Finset α := { σ |  j ∈ A.step i (some σ) }
-    --     let characters := character_set.toList
-
-    --     obtain ⟨ σ, h_step, h_x_σ ⟩ := (character_list_regex_accepts_characters characters (character_list_to_regex characters) rfl x).mp h_r_matches_x
-    --     subst characters character_set
-    --     simp at h_step
-
-    --     use [some σ]
-    --     simp [to_trim, h_x_σ]
-    --     split_ifs
-    --     case pos => simp [h_step]
-    --     case neg => simp [h_step] ; omega
-
-    -- case neg =>
-    --     let rᵢⱼ := regex_for_path_from_i_to_j_through_k A i j (k - 1)
-    --     let rᵢₖ := regex_for_path_from_i_to_j_through_k A i k (k - 1)
-    --     let rₖₖ := regex_for_path_from_i_to_j_through_k A k k (k - 1) -- later: handle kstar
-    --     let rₖⱼ := regex_for_path_from_i_to_j_through_k A k j (k - 1)
-
-    --     simp at h_r_matches_x
-    --     simp [hr, Language.add_def] at h_r_matches_x
-    --     clear hr
-    --     cases h_r_matches_x
-    --     case inl h_x_in_rᵢⱼ =>
-    --         have h_induction := (regex_is_path A i j (k-1) rᵢⱼ rfl x).mp h_x_in_rᵢⱼ
-    --         clear rᵢⱼ rᵢₖ rₖⱼ rₖₖ
-    --         obtain ⟨ x', h_x', h_path ⟩ := h_induction
-
-    --         use x'
-    --         refine ⟨ h_x', ?_ ⟩
-
-    --         have h_contains := regex_for_path_contains_ij A i j k (k-1) (by omega)
-    --         exact εNFA.path_if_contains (to_trim A i j k) (to_trim A i j (k-1)) h_contains i j x' h_path
-    --     case inr h_x_in_rᵢₖ_rₖₖ_rₖⱼ =>
-    --         clear rᵢⱼ
-    --         simp [Language.mul_def] at h_x_in_rᵢₖ_rₖₖ_rₖⱼ
-    --         obtain ⟨ xᵢₖ, h_xᵢₖ, xₖₖ, h_xₖₖ, xₖⱼ, h_xₖⱼ, h_x ⟩ := h_x_in_rᵢₖ_rₖₖ_rₖⱼ
-    --         obtain ⟨ xᵢₖ', h_xᵢₖ', h_path_ik ⟩ := (regex_is_path A i k (k-1) rᵢₖ rfl xᵢₖ).mp h_xᵢₖ
-    --         obtain ⟨ xₖⱼ', h_xₖⱼ', h_path_kj ⟩ := (regex_is_path A k j (k-1) rₖⱼ rfl xₖⱼ).mp h_xₖⱼ
-    --         clear rᵢₖ rₖⱼ h_xᵢₖ h_xₖⱼ
-
-    --         simp [Language.kstar_def] at h_xₖₖ
-    --         obtain ⟨ L, h_L, h_xₖₖ ⟩ := h_xₖₖ
-
-    --         have h_path_L_kk : ∃ (L' : List (List (Option alphabet))), L'.flatten.reduceOption = L.flatten ∧
-    --             (∀ x' ∈ L', Nonempty ((to_trim A k k (k - 1)).Path k k x')) := by
-    --             clear h_L
-    --             induction L
-    --             case nil => use []; simp
-    --             case cons head tail h_induction =>
-    --                 simp at h_xₖₖ
-    --                 obtain ⟨ L'', h_L'', h_path_L'' ⟩ := h_induction h_xₖₖ.right
-    --                 obtain ⟨ head', h_head', h_path_head' ⟩ := (regex_is_path A k k (k-1) rₖₖ rfl head).mp h_xₖₖ.left
-    --                 use head' :: L''
-    --                 simp [List.reduceOption_append, h_head', h_L'', h_path_head']
-    --                 exact h_path_L''
-    --         clear rₖₖ h_xₖₖ
-
-    --         obtain ⟨ L', h_L', h_path_kk ⟩ := h_path_L_kk
-
-    --         let xₖₖ' := L'.flatten
-    --         replace h_path_kk : Nonempty ((to_trim A k k (k - 1)).Path k k xₖₖ') := by
-    --             clear h_L h_L'
-    --             subst xₖₖ'
-    --             induction L'
-    --             case nil => simp only [List.flatten_nil, εNFA.isPath_nil]
-    --             case cons head tail h_induction =>
-    --                 simp at h_path_kk
-    --                 replace h_induction := h_induction h_path_kk.right
-
-    --                 simp [List.flatten_cons]
-    --                 apply (to_trim A k k (k - 1)).isPath_append.mpr
-    --                 exact ⟨ k, h_path_kk.left, h_induction ⟩
-
-    --         use xᵢₖ' ++ xₖₖ' ++ xₖⱼ'
-
-    --         simp [symm h_xᵢₖ', symm h_xₖⱼ'] at h_x
-    --         simp [List.reduceOption_append]
-
-    --         have : xₖₖ'.reduceOption = L.flatten := by
-    --             subst h_L
-    --             simp_all only [xₖₖ']
-
-    --         refine ⟨ by simp_all, ?_ ⟩
-
-    --         have h_containsᵢₖ := regex_for_path_contains_ik A i j k (k-1) (by omega)
-    --         have h_containsₖⱼ := regex_for_path_contains_kj A i j k (k-1) (by omega)
-    --         have h_containsₖₖ := regex_for_path_contains_kk A i j k (k-1) (by omega)
-    --         replace h_path_ik := εNFA.path_if_contains (to_trim A i j k) (to_trim A i k (k-1)) h_containsᵢₖ i k xᵢₖ' h_path_ik
-    --         replace h_path_kj := εNFA.path_if_contains (to_trim A i j k) (to_trim A k j (k-1)) h_containsₖⱼ k j xₖⱼ' h_path_kj
-    --         replace h_path_kk := εNFA.path_if_contains (to_trim A i j k) (to_trim A k k (k-1)) h_containsₖₖ k k xₖₖ' h_path_kk
-
-    --         apply (to_trim A i j k).isPath_append.mpr
-    --         refine ⟨ k, h_path_ik , ?_ ⟩
-    --         apply (to_trim A i j k).isPath_append.mpr
-    --         use k
-
 theorem regex_is_path (A : εNFA α ℕ) (i j k : ℕ) (r: RegularExpression α) (hr: r = regex_for_path_from_i_to_j_through_k A i j k)
     (h_zero_step: ∀ (σ : Option α), A.step 0 σ = ∅) (h_step_zero: ∀ (q : ℕ) (σ : Option α), 0 ∉ A.step q σ):
     ∀ (x : List α), ((x ∈ r.matches') ↔ (∃(x': List (Option α)), (x'.reduceOption = x) ∧
-     ∃ (path_ij: A.Path i j x'), ∀ (k': ℕ), ((k' > k) → k' ∉ path_ij.states.tail))) := by
+     ∃ (path_ij: A.Path i j x'), ∀ (k': ℕ), (k' ∈ path_ij.suppAfterStart → (k' ≤ k)))) := by
     intro x
     constructor
     case mp =>
-        sorry
-        -- exact regex_is_path_mp A i j k r hr h_zero_step h_step_zero x
+        intro h_x_in_r
+        unfold regex_for_path_from_i_to_j_through_k at hr
+        split_ifs at hr
+        case pos h_k_0 h_i_j =>
+            subst h_k_0
+            simp [hr] at h_x_in_r
+            cases h_x_in_r
+            case inl h_x_empty =>
+                simp [Language.one_def] at h_x_empty
+                cases h_i_j
+                case inl h_i_eq_j =>
+                    subst h_i_eq_j
+                    use []
+                    simp only [List.reduceOption_nil, h_x_empty, nonpos_iff_eq_zero, true_and]
+                    obtain ⟨ path_ii ⟩ : Nonempty (A.Path i i []) := A.isPath_nil.mpr rfl
+                    use path_ii
+                    intro k' h_k'
+                    cases path_ii
+                    case nil => simp [Path.suppAfterStart] at h_k'
+                case inr h_step =>
+                    use [none]
+                    simp only [List.reduceOption_cons_of_none, List.reduceOption_nil, h_x_empty, nonpos_iff_eq_zero, true_and]
+                    obtain ⟨ path_ij ⟩ : Nonempty (A.Path i j [none]) := A.isPath_singleton.mpr h_step
+                    use path_ij
+                    intro k' h_k'
+                    cases path_ij
+                    case cons p =>
+                        cases p
+                        case nil => simp [Path.suppAfterStart] at h_k'
+            case inr h_some =>
+                let character_set: Finset α := { σ |  j ∈ A.step i (some σ) }
+                let characters := character_set.toList
+                obtain ⟨ σ, h_step, h_x_σ ⟩ := (character_list_regex_accepts_characters characters (character_list_to_regex characters) rfl x).mp h_some
+                use [some σ]
+                simp only [List.reduceOption_cons_of_some, List.reduceOption_nil, h_x_σ, nonpos_iff_eq_zero, true_and]
+                subst characters character_set
+                simp at h_step
+                obtain ⟨ path_ij ⟩ : Nonempty (A.Path i j [some σ]) := A.isPath_singleton.mpr h_step
+                use path_ij
+                intro k' h_k'
+                cases path_ij
+                case cons p =>
+                    cases p
+                    case nil => simp [Path.suppAfterStart] at h_k'
+
+        case neg h_k_0 h_i_neq_j =>
+            let character_set: Finset α := { σ |  j ∈ A.step i (some σ) }
+            let characters := character_set.toList
+            obtain ⟨ σ, h_step, h_x_σ ⟩ := (character_list_regex_accepts_characters characters (character_list_to_regex characters) rfl x).mp h_some
+            use [some σ]
+            simp only [List.reduceOption_cons_of_some, List.reduceOption_nil, h_x_σ, true_and]
+            subst characters character_set
+            simp at h_step
+            obtain ⟨ path_ij ⟩ : Nonempty (A.Path i j [some σ]) := A.isPath_singleton.mpr h_step
+            use path_ij
+            intro k' h_k'
+            cases path_ij
+            case cons p =>
+                cases p
+                case nil => simp [Path.suppAfterStart] at h_k'
+
+        case neg h_k_neq_0 =>
+            let rᵢⱼ := regex_for_path_from_i_to_j_through_k A i j (k - 1)
+            let rᵢₖ := regex_for_path_from_i_to_j_through_k A i k (k - 1)
+            let rₖₖ := regex_for_path_from_i_to_j_through_k A k k (k - 1) -- later: handle kstar
+            let rₖⱼ := regex_for_path_from_i_to_j_through_k A k j (k - 1)
+
+            simp [hr, Language.add_def] at h_x_in_r
+            clear hr
+            cases h_x_in_r
+            case inl h_x_in_rᵢⱼ =>
+                have h_induction := (regex_is_path A i j (k-1) rᵢⱼ rfl h_zero_step h_step_zero x).mp h_x_in_rᵢⱼ
+                clear rᵢⱼ rᵢₖ rₖⱼ rₖₖ
+                obtain ⟨ x', h_x', path_ij, h_k' ⟩ := h_induction
+
+                use x'
+                refine ⟨ h_x', ?_ ⟩
+                use path_ij
+                intro k' h_supp
+                replace h_k' := h_k' k' h_supp
+                omega
+            case inr h_x_in_rᵢₖ_rₖₖ_rₖⱼ =>
+                clear rᵢⱼ
+                simp [Language.mul_def] at h_x_in_rᵢₖ_rₖₖ_rₖⱼ
+                obtain ⟨ xᵢₖ, h_xᵢₖ, xₖₖ, h_xₖₖ, xₖⱼ, h_xₖⱼ, h_x ⟩ := h_x_in_rᵢₖ_rₖₖ_rₖⱼ
+                obtain ⟨ xᵢₖ', h_xᵢₖ', h_path_ik ⟩ := (regex_is_path A i k (k-1) rᵢₖ rfl h_zero_step h_step_zero xᵢₖ).mp h_xᵢₖ
+                obtain ⟨ xₖⱼ', h_xₖⱼ', h_path_kj ⟩ := (regex_is_path A k j (k-1) rₖⱼ rfl h_zero_step h_step_zero xₖⱼ).mp h_xₖⱼ
+                clear rᵢₖ rₖⱼ h_xᵢₖ h_xₖⱼ
+
+                simp [Language.kstar_def] at h_xₖₖ
+                obtain ⟨ L, h_L, h_xₖₖ ⟩ := h_xₖₖ
+
+                have h_path_L_kk : ∃ (L' : List (List (Option α))), L'.flatten.reduceOption = L.flatten ∧
+                    (∀ x' ∈ L', ∃ (path_kk : A.Path k k x'), ∀ k' ∈ path_kk.suppAfterStart, k' ≤ k - 1) := by
+                    clear h_L
+                    induction L
+                    case nil => use []; simp
+                    case cons head tail h_induction =>
+                        simp at h_xₖₖ
+                        obtain ⟨ L'', h_L'', h_path_L'' ⟩ := h_induction h_xₖₖ.right
+                        obtain ⟨ head', h_head', path_head', h_path_head' ⟩ := (regex_is_path A k k (k-1) rₖₖ rfl h_zero_step h_step_zero head).mp h_xₖₖ.left
+                        use head' :: L''
+                        simp only [List.flatten_cons, List.reduceOption_append, h_head', h_L'', List.mem_cons, forall_eq_or_imp, true_and]
+                        constructor
+                        case left => use path_head'
+                        case right => exact h_path_L''
+                clear rₖₖ h_xₖₖ
+
+                obtain ⟨ L', h_L', h_path_kk ⟩ := h_path_L_kk
+
+                let xₖₖ' := L'.flatten
+                replace h_path_kk : ∃ (path_kk : A.Path k k xₖₖ'), ∀ k' ∈ path_kk.suppAfterStart, k' ≤ k := by
+                    clear h_L h_L'
+                    subst xₖₖ'
+                    induction L'
+                    case nil =>
+                        obtain ⟨ path_kk ⟩ : Nonempty (A.Path k k []) := A.isPath_nil.mpr rfl
+                        use path_kk
+                        intro k' h_supp
+                        simp [Path.suppAfterStart] at h_supp
+                        split at h_supp
+                        case h_1 => trivial
+                        case h_2 => contradiction
+                    case cons head tail h_induction =>
+                        simp only [List.mem_cons, forall_eq_or_imp] at h_path_kk
+                        replace h_induction := h_induction h_path_kk.right
+                        obtain ⟨ path_kk_left,  h_path_kk_left  ⟩ := h_path_kk.left
+                        obtain ⟨ path_kk_right, h_path_kk_right ⟩ := h_induction
+                        use path_kk_left ++ path_kk_right
+
+                        intro k' h_k'
+
+                        sorry
+                        -- cases A.supp_after_start_of_path_append path_kk_left path_kk_right h_k' -- TODO ASK YONATAN
+                        -- case inl h_k'_in_left =>
+                        --     have := h_path_kk_left k' h_k'_in_left
+                        --     omega
+                        -- case inr h_k'_in_right =>
+                        --     replace h_k'_in_right : k' = k ∨ k' ∈ path_kk_right.suppAfterStart := by
+                        --         unfold εNFA.Path.supp at h_k'_in_right
+                        --         split at h_k'_in_right
+                        --         case h_1 => trivial
+                        --         case h_2 =>
+                        --             simp at h_k'_in_right
+                        --             cases h_k'_in_right
+                        --             case inl h => left; exact h
+                        --             case inr h heq =>
+                        --                 right
+                        --                 unfold εNFA.Path.suppAfterStart
+                        --                 split
+                        --                 case h_1 => simp_all
+                        --                 case h_2 =>
+                        --                 sorry
+                        --     cases h_k'_in_right
+                        --     case inl => omega
+                        --     case inr h => exact h_path_kk_right k' h
+
+                use xᵢₖ' ++ xₖₖ' ++ xₖⱼ'
+                simp [symm h_xᵢₖ', symm h_xₖⱼ'] at h_x
+
+                have : xₖₖ'.reduceOption = L.flatten := by
+                    subst h_L
+                    simp_all only [xₖₖ']
+
+                refine ⟨ (by simp_all [List.reduceOption_append]), ?_ ⟩
+
+                obtain ⟨ path_ik, h_path_ik ⟩ := h_path_ik
+                obtain ⟨ path_kk, h_path_kk ⟩ := h_path_kk
+                obtain ⟨ path_kj, h_path_kj ⟩ := h_path_kj
+                use path_ik ++ path_kk ++ path_kj
+                intro k' h_k'
+                cases path_ik
+                case nil =>
+                    cases path_kj
+                    case nil => sorry
+                    case cons => sorry
+                case cons p =>
+                    simp [Path.suppAfterStart] at h_k'
+                    -- have := (supp_of_path_append p (path_kk ++ path_kj)).mp h_k'
+                    -- TODO: Associativity of ++ for paths
+                    sorry
+
     case mpr =>
         intro h
         obtain ⟨ x', h_x', h_path_ij ⟩ := h
-        obtain ⟨ path_ij, h_path_ij ⟩ := h_path_ij
-
-        by_cases k ∈ h_path_ij.supp
-        case pos h_k =>
-            obtain ⟨ stesp_ik, steps_kk, steps_kj, h_steps ⟩ := split_path_by_state A i j k x' path_ij h_k
-
-
-            sorry
-        case neg =>
-            -- by induction r₁
-            sorry
-
-        -- unfold regex_for_path_from_i_to_j_through_k at hr
-
-        -- split_ifs at hr
-        -- case pos h_k_0 h_ij => sorry
-        --     subst h_ij h_k_0
-        --     simp at hr
-        --     subst hr
-        --     induction x' generalizing x
-        --     case nil =>
-        --         simp at h_x'
-        --         subst h_x'
-        --         simp [Language.kstar_def]
-        --         use []
-        --         simp
-        --     case cons c tail h_induction =>
-        --         have h_tail_path : Nonempty ((to_trim A i i 0).Path i i tail) := by
-        --             by_cases h_i_0: i = 0
-        --             case pos =>
-        --                 subst h_i_0
-        --                 obtain ⟨ h_x'_path ⟩ := h_x'_path
-        --                 cases h_x'_path
-        --                 case cons t h_step h_path =>
-        --                     simp [to_trim] at h_step
-        --                     simp [h_step.right] at h_path
-        --                     use h_path
-        --             case neg =>
-        --                 obtain ⟨ h_x'_path ⟩ := h_x'_path
-        --                 cases h_x'_path
-        --                 case cons t h_step h_path =>
-        --                     replace h_i_0: i > 0 := by omega
-        --                     simp [to_trim, h_i_0] at h_step
-        --                     cases h_step
-        --                     case inl h_t_0 =>
-        --                         have := h_t_0.right
-        --                         subst this
-        --                         simp at h_t_0
-
-        --                         cases h_path
-        --                         case nil => simp
-        --                         case cons _ _ _ h_step' _ =>
-        --                             unfold to_trim at h_step'
-        --                             split_ifs at h_step'
-        --                             simp at h_step'
-        --                             cases h_step'
-        --                             case inl h_t'_0 =>
-        --                                 simp [h_t'_0.right, h_zero_step] at h_t'_0 --contradiction
-        --                             case inr h_t'_i =>
-        --                                 simp [h_t'_i.right, h_zero_step] at h_t'_i --contradiction
-
-        --                     case inr h_t_i =>
-        --                         simp [h_t_i.right] at h_path
-        --                         use h_path
-
-        --         by_cases c = none
-        --         case pos h_c_none =>
-        --             subst h_c_none
-        --             exact h_induction x h_x' h_tail_path
-        --         case neg h_c_some =>
-        --             have h_step: i ∈ (to_trim A i i 0).step i c := by
-        --                 obtain ⟨ h_x'_path ⟩ := h_x'_path
-        --                 cases h_x'_path
-        --                 case cons t h_step h_path =>
-        --                     simp [to_trim] at h_step
-        --                     split_ifs at h_step
-        --                     case pos h_i =>
-        --                         simp at h_step
-        --                         cases h_step
-        --                         case inl h_t_0 =>
-        --                             have := h_t_0.right
-        --                             subst this
-        --                             cases h_path
-        --                             case nil => simp [h_zero_step] at h_t_0 -- contradiction
-        --                             case cons _ _ _ h_step' _ =>
-        --                                 simp [to_trim] at h_step'
-        --                                 split_ifs at h_step'
-        --                                 simp at h_step'
-        --                                 cases h_step'
-        --                                 case inl h_step' =>
-        --                                     simp [h_zero_step] at h_step' -- contradiction
-        --                                 case inr h_step' =>
-        --                                     simp [h_zero_step] at h_step' -- contradiction
-
-        --                         case inr h_t_i =>
-        --                             simp [h_t_i.right] at h_t_i
-        --                             simp [to_trim, h_i]
-        --                             right
-        --                             exact h_t_i
-
-        --                     case neg h_i =>
-        --                         replace h_i : i = 0 := by omega
-        --                         subst h_i
-        --                         simp [h_zero_step] at h_step --contradiction
-
-        --             replace h_induction := h_induction tail.reduceOption rfl h_tail_path
-        --             simp [Language.kstar_def] at h_induction ⊢
-        --             obtain ⟨ L, h_L_tail, h_L_matches ⟩ := h_induction
-
-        --             replace h_c_some := not_none_is_some c h_c_some
-        --             obtain ⟨ σ, h_σ ⟩ := h_c_some
-        --             subst h_σ
-
-        --             use [σ] :: L
-        --             simp [h_L_tail] at h_x'
-        --             simp
-        --             refine ⟨ symm h_x', ?_, h_L_matches ⟩
-        --             simp [to_trim] at h_step
-        --             split_ifs at h_step
-        --             case pos h_i_0 =>
-        --                 replace h_i_0 : i ≠ 0 := by omega
-        --                 simp [h_i_0] at h_step
-        --                 let character_set: Finset α := { σ |  i ∈ A.step i (some σ) }
-        --                 let characters := character_set.toList
-        --                 let r := character_list_to_regex characters
-
-        --                 apply (character_list_regex_accepts_characters characters r rfl [σ]).mpr
-        --                 use σ
-        --                 subst characters character_set
-        --                 simp
-        --                 exact h_step
-        --             case neg h_i_0 =>
-        --                 replace h_i_0 : i = 0 := by omega
-        --                 subst h_i_0
-        --                 simp [h_zero_step] at h_step --contradiction
-
-        -- case pos h_k_0 h_i_neq_j h_step =>
-        --     cases x'
-        --     case nil =>
-        --         subst h_x' hr
-        --         simp [Language.mem_add, Language.mem_mul]
-        --         left
-        --         simp [Language.kstar_def]
-        --         use []
-        --         simp
-        --     case cons c tail =>
-        --         subst hr
-        --         simp [Language.mem_add, Language.mem_mul]
-        --         by_cases c = none
-        --         case pos h_c_none =>
-        --             left
-        --             subst h_c_none
-        --             simp at h_x'
-        --             obtain ⟨ h_x'_path ⟩ := h_x'_path
-        --             cases h_x'_path
-        --             case cons t h_step h_path =>
-        --                 let character_set: Finset α := { σ | j ∈ A.step j (some σ) }
-        --                 let characters := character_set.toList
-        --                 let r := character_list_to_regex characters
-        --                 have h_t_j : j = t := by
-        --                     subst h_k_0
-        --                     unfold to_trim at h_step
-        --                     simp at h_step
-        --                     split_ifs at h_step
-        --                     case pos =>
-        --                         simp at h_step
-        --                         cases h_step
-        --                         case inl h =>
-        --                             obtain ⟨ h_step', h_t_0 ⟩ := h
-        --                             subst h_t_0
-        --                             cases h_path
-        --                             case nil => rfl
-        --                             case cons _ σ' _ h_step' _ =>
-        --                                 simp [to_trim] at h_step'
-        --                                 simp_all
-        --                         case inr h => exact symm h.right
-        --                     case neg =>
-        --                         simp at h_step
-        --                         obtain ⟨ h_step', h_t_0 ⟩ := h_step
-        --                         subst h_t_0
-        --                         cases h_path
-        --                         case nil => rfl
-        --                         case cons _ σ' _ h_step' _ =>
-        --                             simp [to_trim] at h_step'
-        --                             simp_all
-
-        --                 subst h_t_j
-        --                 simp [Language.kstar_def]
-        --                 induction tail generalizing x
-        --                 case nil =>
-        --                     simp at h_x'
-        --                     use []
-        --                     simp [h_x']
-        --                 case cons c' tail' h_induction =>
-        --                     rw [← List.singleton_append] at h_path
-        --                     replace h_path : Nonempty ((to_trim A i j k).Path j j ([c'] ++ tail')) := by use h_path
-        --                     obtain ⟨ t, h_path_c, h_path_tail' ⟩ := (to_trim A i j k).isPath_append.mp h_path
-
-        --                     have h_t_j : j = t := by
-        --                         simp [to_trim, h_k_0] at h_path_c
-        --                         split_ifs at h_path_c
-        --                         case pos =>
-        --                             simp at h_path_c
-        --                             cases h_path_c
-        --                             case inl h =>
-        --                                 obtain ⟨ h_step_t, h_t_0 ⟩ := h
-        --                                 subst h_t_0
-        --                                 have := h_step_zero j c'
-        --                                 contradiction
-        --                             case inr h =>
-        --                                 obtain ⟨ h_step_t, h_t_j ⟩ := h
-        --                                 exact symm h_t_j
-        --                         case neg =>
-        --                             simp at h_path_c
-        --                             obtain ⟨ h_step_t, h_t_0 ⟩ := h_path_c
-        --                             subst h_t_0
-        --                             have := h_step_zero j c'
-        --                             contradiction
-
-        --                     subst h_t_j
-
-        --                     obtain ⟨ h_path_tail' ⟩ := h_path_tail'
-        --                     have := h_induction tail'.reduceOption rfl h_path_tail'
-        --                     obtain ⟨ L', h ⟩ := this
-        --                     cases c'
-        --                     case none =>
-        --                         use L'
-        --                         simp at h_x'
-        --                         subst h_x'
-        --                         exact h
-        --                     case some σ =>
-        --                         use [σ] :: L'
-        --                         simp [h.left] at h_x'
-        --                         simp [h_x']
-        --                         refine ⟨ ?_, h.right ⟩
-        --                         simp [to_trim, h_k_0] at h_path_c
-        --                         split_ifs at h_path_c
-        --                         case pos =>
-        --                             simp at h_path_c
-        --                             cases h_path_c
-        --                             case inl => omega -- contradiction
-        --                             case inr h =>
-        --                                 have : σ ∈ characters := by
-        --                                     unfold characters character_set
-        --                                     simp [h]
-        --                                 exact (character_list_regex_accepts_characters characters r rfl [σ]).mpr ⟨ σ, this, rfl ⟩
-        --                         case neg =>
-        --                             simp at h_path_c
-        --                             obtain ⟨ h_step, h_j_0 ⟩ := h_path_c
-        --                             subst h_j_0
-        --                             have := h_zero_step (some σ)
-        --                             simp [this] at h_step -- contradiction
-
-        --         case neg h_c_some =>
-        --             right
-        --             clear h_step
-        --             replace h_c_some := not_none_is_some c h_c_some
-        --             obtain ⟨ σ, h_σ ⟩ := h_c_some
-        --             subst h_σ
-        --             simp at h_x'
-
-        --             obtain ⟨ h_x'_path ⟩ := h_x'_path
-        --             cases h_x'_path
-        --             case cons t h_step h_path =>
-        --                 have h_t_j : j = t := by
-        --                     simp [to_trim, h_k_0] at h_step
-        --                     split_ifs at h_step
-        --                     case pos =>
-        --                         simp at h_step
-        --                         cases h_step
-        --                         case inl h =>
-        --                             obtain ⟨ h_step_t, h_t_0 ⟩ := h
-        --                             subst h_t_0
-        --                             have := h_step_zero i (some σ)
-        --                             contradiction
-        --                         case inr h =>
-        --                             obtain ⟨ h_step_t, h_t_j ⟩ := h
-        --                             exact symm h_t_j
-        --                     case neg =>
-        --                         simp at h_step
-        --                         obtain ⟨ h_step_t, h_t_0 ⟩ := h_step
-        --                         subst h_t_0
-        --                         have := h_step_zero i (some σ)
-        --                         contradiction
-        --                 subst h_t_j
-
-        --                 use [σ]
-        --                 simp
-        --                 constructor
-        --                 case left =>
-        --                     let character_set: Finset α := { σ | j ∈ A.step i (some σ) }
-        --                     let characters := character_set.toList
-        --                     let r := character_list_to_regex characters
-
-        --                     have : σ ∈ characters := by
-        --                         unfold characters character_set
-        --                         simp [to_trim] at h_step
-        --                         subst h_k_0
-        --                         split_ifs at h_step
-        --                         case pos =>
-        --                             simp at h_step ⊢
-        --                             cases h_step
-        --                             case inl h => exact h.left
-        --                             case inr h => exact h
-        --                         case neg =>
-        --                             simp at h_step ⊢
-        --                             exact h_step.left
-
-        --                     exact (character_list_regex_accepts_characters characters r rfl [σ]).mpr ⟨ σ, this, rfl ⟩
-
-        --                 case right =>
-        --                     induction tail generalizing x
-        --                     case nil =>
-        --                         simp at h_x'
-        --                         use []
-        --                         simp [h_x', Language.kstar_def]
-        --                         use []
-        --                         simp
-
-        --                     case cons c' tail' h_induction =>
-        --                         rw [← List.singleton_append] at h_path
-        --                         replace h_path : Nonempty ((to_trim A i j k).Path j j ([c'] ++ tail')) := by use h_path
-        --                         have := (to_trim A i j k).isPath_append.mp h_path
-        --                         obtain ⟨ t, h_path_c, h_path_tail' ⟩ := this
-        --                         have h_t_j : j = t := by sorry --TODO!!!
-        --                         subst h_t_j
-        --                         obtain ⟨ h_path_tail' ⟩ := h_path_tail'
-        --                         have := h_induction (σ :: tail'.reduceOption) rfl h_path_tail'
-        --                         obtain ⟨ b, h_b, h_tail' ⟩ := this
-        --                         simp at h_tail' h_x'
-
-        --                         cases c'
-        --                         case none =>
-        --                             use b
-        --                             simp at h_x'
-        --                             subst h_x' h_tail'
-        --                             simp
-        --                             exact h_b
-        --                         case some σ =>
-        --                             use σ :: b
-        --                             simp at h_x'
-        --                             subst h_x' h_tail'
-        --                             simp
-
-        --                             simp [to_trim, h_k_0] at h_path_c
-        --                             split_ifs at h_path_c
-        --                             case pos =>
-        --                                 simp at h_path_c
-        --                                 cases h_path_c
-        --                                 case inl => omega -- contradiction
-        --                                 case inr h =>
-        --                                     let character_set: Finset α := { σ | j ∈ A.step j (some σ) }
-        --                                     let characters := character_set.toList
-        --                                     let r := character_list_to_regex characters
-        --                                     have : σ ∈ characters := by
-        --                                         unfold characters character_set
-        --                                         simp [h]
-        --                                     replace := (character_list_regex_accepts_characters characters r rfl [σ]).mpr ⟨ σ, this, rfl ⟩
-
-        --                                     simp [Language.kstar_def] at h_b ⊢
-        --                                     obtain ⟨ L', h_L' ⟩ := h_b
-        --                                     use [σ] :: L'
-        --                                     subst character_set characters r
-        --                                     simp [h_L', this]
-        --                                     exact h_L'.right
-
-        --                             case neg =>
-        --                                 simp at h_path_c
-        --                                 obtain ⟨ h_step, h_j_0 ⟩ := h_path_c
-        --                                 subst h_j_0
-        --                                 have := h_zero_step (some σ)
-        --                                 simp [this] at h_step -- contradiction
-
-        case neg h_k_0 h_i_neq_j h_not_step => sorry
-            -- cases x'
-            -- case nil =>
-            --     simp at h_x'_path
-            --     contradiction
-            -- case cons c tail =>
-            --     rw [← List.singleton_append] at h_x'_path
-            --     obtain ⟨ t, h_path_c, h_path' ⟩ := (to_trim A i j k).isPath_append.mp h_x'_path
-            --     simp [to_trim, h_k_0] at h_path_c
-            --     split_ifs at h_path_c
-            --     case pos =>
-            --         simp at h_path_c
-            --         cases h_path_c
-            --         case inl h_t_0 => simp_all [h_t_0.right]
-            --         case inr h_t_j =>
-            --             obtain ⟨ h_step_t, h_t_j ⟩ := h_t_j
-            --             symm at h_t_j
-            --             subst h_t_j
-
-            --             have : ∃ σ, c = some σ := by
-            --                 apply not_none_is_some
-            --                 by_contra!
-            --                 subst this
-            --                 contradiction
-            --             obtain ⟨ σ, h_σ ⟩ := this
-            --             subst h_σ
-
-            --             simp at h_x'_path
-            --             subst hr
-            --             simp
-            --             simp at h_x'
-            --             subst h_x'
-            --             rw [← List.singleton_append] at h_x'_path
-            --             obtain ⟨ t, h_path_σ, h_path_tail ⟩ := (to_trim A i j k).isPath_append.mp h_x'_path
-            --             clear h_x'_path
-            --             have h_t_j : j = t := by
-            --                 simp [to_trim, h_k_0] at h_path_σ
-            --                 split_ifs at h_path_σ
-            --                 simp at h_path_σ
-            --                 cases h_path_σ
-            --                 case inl h =>
-            --                     obtain ⟨ h_step_t, h_t_0 ⟩ := h
-            --                     subst h_t_0
-            --                     have := h_step_zero i (some σ)
-            --                     contradiction
-            --                 case inr h =>
-            --                     obtain ⟨ h_step_t, h_t_j ⟩ := h
-            --                     exact symm h_t_j
-            --             subst h_t_j
-
-            --             let character_set_ij: Finset α := { σ | j ∈ A.step i (some σ) }
-            --             let characters_ij := character_set_ij.toList
-            --             let r_ij := character_list_to_regex characters_ij
-
-            --             have h_matches_σ : σ ∈ characters_ij := by
-            --                 simp [to_trim, h_k_0] at h_path_σ
-            --                 split_ifs at h_path_σ
-            --                 simp at h_path_σ
-            --                 simp [characters_ij, character_set_ij]
-            --                 cases h_path_σ
-            --                 case inl h => exact h.left
-            --                 case inr h => exact h
-
-            --             replace h_matches_σ := (character_list_regex_accepts_characters characters_ij r_ij rfl [σ]).mpr ⟨ σ, h_matches_σ, rfl ⟩
-            --             simp [Language.mem_mul]
-            --             use [σ]
-            --             refine ⟨ h_matches_σ, ?_ ⟩
-
-            --             induction tail
-            --             case nil =>
-            --                 use []
-            --                 simp [Language.kstar_def]
-            --                 use []
-            --                 simp
-
-            --             case cons c' tail' h_induction =>
-            --                 clear h_path_tail
-            --                 rw [← List.singleton_append] at h_path'
-            --                 obtain ⟨ t, h_path_c', h_path_tail' ⟩ := (to_trim A i j k).isPath_append.mp h_path'
-            --                 have h_t_j : j = t := by
-            --                     simp [to_trim, h_k_0] at h_path_c'
-            --                     split_ifs at h_path_c'
-            --                     simp at h_path_c'
-            --                     cases h_path_c'
-            --                     case inl h =>
-            --                         obtain ⟨ h_step_t, h_t_0 ⟩ := h
-            --                         subst h_t_0
-            --                         have := h_step_zero j c'
-            --                         contradiction
-            --                     case inr h =>
-            --                         obtain ⟨ h_step_t, h_t_j ⟩ := h
-            --                         exact symm h_t_j
-            --                 subst h_t_j
-
-            --                 have := h_induction h_path_tail' h_path_tail'
-            --                 simp [Language.kstar_def] at this ⊢
-            --                 obtain ⟨ L', h_L' ⟩ := this
-
-            --                 cases c'
-            --                 case none =>
-            --                     simp
-            --                     use L'
-            --                 case some σ' =>
-            --                     use [σ'] :: L'
-            --                     simp
-            --                     refine ⟨ h_L'.left , ?_, h_L'.right ⟩
-
-            --                     let character_set_jj: Finset α := { σ | j ∈ A.step j (some σ) }
-            --                     let characters_jj := character_set_jj.toList
-            --                     let r_jj := character_list_to_regex characters_jj
-
-            --                     have h_matches_σ' : σ' ∈ characters_jj := by
-            --                         simp [to_trim, h_k_0] at h_path_c'
-            --                         split_ifs at h_path_c'
-            --                         simp at h_path_c'
-            --                         simp [characters_jj, character_set_jj]
-            --                         cases h_path_c'
-            --                         case inl h => exact h.left
-            --                         case inr h => exact h
-
-            --                     exact (character_list_regex_accepts_characters characters_jj r_jj rfl [σ']).mpr ⟨ σ', h_matches_σ', rfl ⟩
-
-            --     case neg h_j_0 =>
-            --         simp at h_j_0
-            --         subst h_j_0
-            --         simp at h_path_c
-            --         obtain ⟨ h_step, h_t_0 ⟩ := h_path_c
-            --         subst h_t_0
-            --         have := h_step_zero i c
-            --         contradiction
-
-        -- case neg h_k_not_0 =>
-        --     let rᵢⱼ := regex_for_path_from_i_to_j_through_k A i j (k - 1)
-        --     let rᵢₖ := regex_for_path_from_i_to_j_through_k A i k (k - 1)
-        --     let rₖₖ := regex_for_path_from_i_to_j_through_k A k k (k - 1)
-        --     let rₖⱼ := regex_for_path_from_i_to_j_through_k A k j (k - 1)
-
-        --     let A_ij := (to_trim A i j k)
-        --     let A_ik := (to_trim A i k (k - 1))
-        --     let A_kk := (to_trim A k k (k - 1))
-        --     let A_kj := (to_trim A k j (k - 1))
-
-        --     have h_path_ij : Nonempty (A_ij.Path i j x') := h_x'_path
-        --     obtain ⟨ path_ij ⟩ := h_path_ij
-
-        --     simp [hr]
-        --     by_cases k ∈ path_ij.supp
-        --     case pos h_k_supp =>
-        --         right
-        --         have h_lemma : ∃ (x'_ik x'_kk x'_kj : List (Option α)),
-        --             Nonempty (A_ik.Path i k x'_ik) ∧
-        --             (∃ (L' : List (List (Option α))), L'.flatten = x'_kk ∧
-        --              ∀ y' ∈ L', Nonempty (A_kk.Path k k y')) ∧
-        --             Nonempty (A_kj.Path k j x'_kj) ∧
-        --             x' = x'_ik ++ x'_kk ++ x'_kj := by
-
-        --             have h_x'_ik : ∃ (x'_ik : List (Option α)), x'_ik.isPrefixOf x' ∧
-        --                 ((i = k ∧ x'_ik = []) ∨ ∃ (path_ik : A_ij.Path i k x'_ik), k ∉ path_ik.supp) := by
-        --                 have := path_prefix_of_state A_ij i j k x' path_ij h_k_supp
-        --                 cases this
-        --                 case inl h_ik =>
-        --                     subst h_ik
-        --                     use []
-        --                     simp
-        --                 case inr h_y' =>
-        --                     obtain ⟨ y', h_y'_prefix, path_ik, h_path_ik ⟩ := h_y'
-        --                     use y'
-        --                     simp [h_y'_prefix]
-        --                     right
-        --                     use path_ik
-
-        --             obtain ⟨ x'_ik, h_prefix, h ⟩ := h_x'_ik
-
-        --             use x'_ik
-        --             have : Nonempty (A_ik.Path i k x'_ik) := by
-        --                 cases h
-        --                 case inl h =>
-        --                     obtain ⟨ h_ik, h_empty ⟩ := h
-        --                     subst h_ik h_empty
-        --                     apply A_ik.isPath_nil.mpr
-        --                     rfl
-        --                 case inr h_path_ik =>
-        --                     obtain ⟨ path_ik , h_k_notin_supp ⟩ := h_path_ik
-        --                     have := path_trim_of_not_mem_supp A i j k i k x'_ik h_k_not_0 path_ik h_k_notin_supp
-
-        --                     -- have h_x_in_left : Nonempty ((to_trim A i j (k - 1)).Path i j x') :=
-        --                     --     path_trim_of_not_mem_supp A i j k i j x' h_k_not_0 path_ij h_k_notin_supp
-
-        --                     sorry
-        --             sorry
-
-        --         simp [Language.mul_def]
-        --         obtain ⟨ x'_ik, x'_kk, x'_kj, h_x'', h_x'_ik, h_x'_kk, h_x'_kj ⟩ := h_lemma
-
-        --         refine ⟨ x'_ik.reduceOption, ?_, x'_kk.reduceOption, ?_, x'_kj.reduceOption, ?_, ?_ ⟩
-        --         case refine_1 =>
-        --             exact (regex_is_path A i k (k - 1) rᵢₖ rfl
-        --                 h_zero_step h_step_zero x'_ik.reduceOption).mpr
-        --                 ⟨x'_ik, rfl, h_x'_ik⟩
-
-        --         case refine_2 =>
-        --             simp [Language.kstar_def]
-        --             obtain ⟨ L', h_L'_x'_kk, h_L' ⟩ := h_x'_kk
-        --             let L : List (List α) := L'.map (fun x' => x'.reduceOption)
-        --             use L
-        --             refine ⟨ ?_, ?_ ⟩
-        --             case refine_1 =>
-        --                 subst h_L'_x'_kk L
-        --                 exact list_map_of_reduce_option L'
-
-        --             case refine_2 =>
-        --                 intro y h_y
-        --                 have : ∃ y' ∈ L', y'.reduceOption = y := by
-        --                     subst L
-        --                     simp at h_y
-        --                     exact h_y
-        --                 obtain ⟨ y', h_y'_in_L', h_y' ⟩ := this
-        --                 have := h_L' y' h_y'_in_L'
-
-        --                 exact (regex_is_path A k k (k - 1) rₖₖ rfl
-        --                     h_zero_step h_step_zero y).mpr
-        --                     ⟨y', h_y', this⟩
-
-        --         case refine_3 =>
-        --             exact (regex_is_path A k j (k - 1) rₖⱼ rfl
-        --                 h_zero_step h_step_zero x'_kj.reduceOption).mpr
-        --                 ⟨x'_kj, rfl, h_x'_kj⟩
-
-        --         case refine_4 =>
-        --             have : x'.reduceOption = x'_ik.reduceOption ++ x'_kk.reduceOption ++ x'_kj.reduceOption := by
-        --                 subst h_x''
-        --                 simp [List.reduceOption_append]
-        --             subst h_x'
-        --             simp [this]
-
-        --     case neg h_k_notin_supp =>
-        --         left
-        --         have h_x_in_left : Nonempty ((to_trim A i j (k - 1)).Path i j x') :=
-        --             path_trim_of_not_mem_supp A i j k i j x' h_k_not_0 path_ij h_k_notin_supp
-
-        --         exact (regex_is_path A i j (k - 1) rᵢⱼ rfl
-        --             h_zero_step h_step_zero x).mpr
-        --             ⟨x', h_x', h_x_in_left⟩
-
-            --cases h_x'_path
-
-            -- by_cases Nonempty ((to_trim A i j (k - 1)).Path i j x')
-            -- case pos h_x_in_left =>
-            --     left
-            --     exact (regex_is_path A i j (k-1) rᵢⱼ rfl h_zero_step h_step_zero x).mpr ⟨ x', h_x', h_x_in_left ⟩
-            -- case neg h_x_not_in_left =>
-            --     right
-            --     simp [Language.mul_def]
-
-            --     have h_x_decomposition : ∃ (x_ik x_kk x_kj : List α), x = x_ik ++ x_kk ++ x_kj ∧
-            --         x_ik ∈ rᵢₖ.matches' ∧ x_kk ∈ rₖₖ.star.matches' ∧ x_kj ∈ rₖⱼ.matches' := by
-            --         induction x'
-            --         case nil =>
-            --             use [], [], []
-            --             simp at h_x'
-            --             simp [h_x']
-            --             sorry
-            --         case cons c tail h_induction =>
-
-
-            --         unfold to_trim at h_x'_path
-            --         split_ifs at h_x'_path
-            --         case pos h_k_greater_than_j =>
-            --             simp at h_x'_path
-            --             cases h_x'_path
-            --             sorry
-            --         case neg h_k_leq_than_j =>
-            --             sorry
-
-            --     obtain ⟨ x_ik, x_kk, x_kj, h_x, h_x_ik, h_x_kk, h_x_kj ⟩ := h_x_decomposition
-            --     use x_ik
-            --     refine ⟨ h_x_ik , ?_ ⟩
-            --     use x_kk
-            --     refine ⟨ h_x_kk , ?_ ⟩
-            --     use x_kj
-            --     refine ⟨ h_x_kj, ?_ ⟩
-            --     simp [h_x]
+        obtain ⟨ path_ij, h_k ⟩ := h_path_ij
+
+        by_cases k ∈ path_ij.supp
+        case pos h_k_in_supp =>
+            unfold regex_for_path_from_i_to_j_through_k at hr
+            split_ifs at hr
+            case pos h_k_0 h_i_j =>
+                subst h_k_0
+                sorry
+            case neg h_k_0 h =>
+                sorry
+            case neg h_k_neq_0 =>
+                obtain ⟨ p ⟩ := path_multiple_split_at_state A i j k x' path_ij h_k_in_supp
+                obtain ⟨ word_ik, word_kk, word_kj, path_ik, path_kk, path_kj,
+                        h_word_ij, h_path_ij, h_k_notin_ik, h_k_notin_kj ⟩ := p
+                subst hr
+                simp [Language.add_def]
+                right
+                simp [Language.mul_def]
+                use word_ik.reduceOption
+                refine ⟨ ?_, ?_ ⟩
+                case refine_1 =>
+                    exact (regex_is_path A i k (k - 1) (regex_for_path_from_i_to_j_through_k A i k (k - 1))
+                        rfl h_zero_step h_step_zero word_ik.reduceOption).mpr ⟨ word_ik, rfl, path_ik, sorry ⟩
+
+                use word_kk.reduceOption
+                refine ⟨ ?_, ?_ ⟩
+                case refine_1 =>
+                    simp [Language.kstar_def]
+                    use [word_kk.reduceOption]
+                    simp
+                    -- TODO: Not correct, need to split word_kk into words that don't pass through k
+                    exact (regex_is_path A k k (k - 1) (regex_for_path_from_i_to_j_through_k A k k (k - 1))
+                        rfl h_zero_step h_step_zero word_kk.reduceOption).mpr ⟨ word_kk, rfl, path_kk, sorry ⟩
+
+                use word_kj.reduceOption
+                refine ⟨ ?_, ?_ ⟩
+                case refine_1 =>
+                    exact (regex_is_path A k j (k - 1) (regex_for_path_from_i_to_j_through_k A k j (k - 1))
+                        rfl h_zero_step h_step_zero word_kj.reduceOption).mpr ⟨ word_kj, rfl, path_kj, sorry ⟩
+
+                subst h_word_ij
+                simp [List.reduceOption_append] at h_x'
+                exact h_x'
+
+        case neg h_k_notin_supp =>
+            subst hr
+            unfold regex_for_path_from_i_to_j_through_k
+            split_ifs
+            case pos h_k_0 h_i_j =>
+                cases h_i_j
+                case inl h_i_j =>
+                    subst h_i_j
+                    have : x'.length ≤ 1 := by
+                        by_contra!
+                        cases path_ij
+                        case nil => contradiction
+                        case cons => sorry
+
+                    simp [Language.add_def, Language.one_def]
+                    by_cases x'.length = 0
+                    case pos h_x'_0 =>
+                        left
+                        simp at h_x'_0
+                        subst h_x'_0
+                        simp at h_x'
+                        exact h_x'
+                    case neg h_x'_1 =>
+                        replace h_x'_1 : x'.length = 1 := by omega
+                        obtain ⟨ σ, h_σ ⟩ := x'.length_eq_one_iff.mp h_x'_1
+                        cases σ
+                        case none =>
+                            left
+                            subst h_σ
+                            simp at h_x'
+                            exact h_x'
+                        case some c =>
+                            right
+                            cases path_ij
+                            case nil => contradiction
+                            case cons _ c' _ h_step p =>
+                                simp at h_x'_1
+                                subst h_x'_1
+                                have := (A.isPath_nil.mp (by use p)).symm
+                                simp at h_σ
+                                subst this h_σ
+
+                                let character_set: Finset α := { σ | i ∈ A.step i (some σ) }
+                                let characters := character_set.toList
+
+                                have h_c : c ∈ characters := by
+                                    subst characters character_set
+                                    simp [h_step]
+
+                                simp at h_x'
+
+                                exact (character_list_regex_accepts_characters characters
+                                       (character_list_to_regex characters) rfl x).mpr ⟨c, h_c, h_x'.symm⟩
+                case inr h_step => sorry
+
+            case neg h_k_0 h => sorry
+            case neg h_k_neq_0 =>
+                simp [Language.add_def]
+                left
+
+                have : ∀ k' ∈ path_ij.suppAfterStart, k' ≤ (k-1) := by
+                    intro k' h_k'
+                    replace h_k := h_k k' h_k'
+                    have : k' ≠ k := by
+                        by_contra!
+                        subst this
+                        have : k' ∉ path_ij.suppAfterStart := by
+                            by_contra!
+                            have := if_supp_after_start_then_supp path_ij
+                            sorry
+                        contradiction
+                    omega
+
+                exact (regex_is_path A i j (k - 1) (regex_for_path_from_i_to_j_through_k A i j (k - 1))
+                            rfl h_zero_step h_step_zero x).mpr ⟨ x', h_x', path_ij, this ⟩
 
 theorem εNFA_to_Regex (A: εNFA α ℕ) : A.is_finite_automata → (∃ (r: RegularExpression α), r.matches' = A.accepts) := by
     sorry
